can't do  Lemma picomp2_works: forall G T1 T2 T3,   tr     [:: hyp_tm           (sigma nattp              (prod                 (prod                    T1                   T2)                 T3)), hyp_tm preworld       & G] cuz need to restrict the T from referring to var 1

help.v
@@ -58,7 +58,7 @@ Definition Yc: (term False) := lam ((*f := 0*)
 (*Computation monad*)
 Definition ret: term False := lam (inl (var 0)).
 
-Definition ret_t x := app ret x.
+Definition ret_a x := app ret x.
 
 Definition bind : term False := app Yc
    (lam   ( (*f := 0*)
